## Higher Order DE
1.
$$ (D^2 - 3D + 2)y = e^{3x}   \space \space; \space \space \space \space \space y(x) = c_1 e^x + c_2 e^{2x} + \frac{e^{3x}}{2} $$

2.
$$ (D^2 - 4D + 3)y = e^{2x} \space \space; \space \space \space \space \space y(x) = c_1 e^x + c_2 e^{3x} - e^{2x} $$

3.
$$ \frac{d^2y}{dx^2} - 4y = e^{2x} + 3e^{-2x} + 7e^x \space \space; \space \space y(x) = c_1 e^{2x} + c_2 e^{-2x} + \frac{xe^{2x}}{4} - \frac{3xe^{-2x}}{4} - \frac{7e^x}{3} $$

4. 
$$ \frac{d^3y}{dx^3} - 3 \frac{d^2y}{dx^2} + 3 \frac{dy}{dx} - y = e^x - 3e^{-2x} \space \space; \space \space y(x) = (c_1 + c_2 x + c_3 x^2)e^x + \frac{e^x x^3}{6} + \frac{e^{-2x}}{9} $$

5.
$$ \frac{d^2y}{dx^2} + 2 \frac{dy}{dx} + 2y = e^{3x} - 4e^{-x} + 5 \space \space; \space \space y(x) = e^{-x} \left( c_1 \cos x + c_2 \sin x \right) + \frac{e^{3x}}{17} - 4e^{-x} + \frac{5}{2} $$

6.
$$ (D^3 + 8)y = 4 + e^{-2x} \space \space; \space \space y(x) = e^x \left( c_1 \cos(\sqrt{3} \space x) + c_2 \sin(\sqrt{3} \space x) \right) + c_3 e^{-2x} + \frac{1}{2} + \frac{xe^{-2x}}{12} $$

7.
$$ (D+2)(D-1)^2 y = e^{-2x} + 2 \sinh x \space \space; \space \space y(x) = c_1 e^{-2x} + (c_2 + c_3 x)e^x + \frac{xe^{-2x}}{9} + \frac{x^2 e^x}{6} - \frac{e^{-x}}{4} $$

8.
$$ (D^2 - 4)y = \sin x \space \space; \space \space y(x) = c_1 e^{-2x} + c_2 e^{2x} - \frac{\sin x}{5} $$

9.
$$ (D^2 + 4)y = \cos 2x \space \space; \space \space y(x) = c_1 \cos 2x + c_2 \sin 2x + \frac{x \sin 2x}{4} $$

10.
$$ (D^4 - 3D^2 - 4)y = 5 \sin 2x - e^{-2x} \quad ; \quad c_1 e^{2x} + c_2 e^{-2x} + c_3 \cos x + c_4 \sin x + \frac{5 \sin 2x}{24} + \frac{xe^{-2x}}{20} $$

11. 
$$ (D^2 + 2D + 1)y = 4 \sin 2x \space \space; \space \space y(x) = (c_1 + c_2 x)e^{-x} - \frac{4(4 \cos 2x + 3 \sin 2x)}{25} $$

12.
$$ \frac{d^3y}{dx^3} + 4 \frac{dy}{dx} = \sin 2x \space \space; \space \space y(x) = c_1 + (c_2 \cos 2x + c_3 \sin 2x) - \frac{x \sin 2x}{8} $$

13.
$$ (D^2 + 1)y = \sin x \sin 2x \space \space; \space \space y(x) = (c_1 \cos 2x + c_2 \sin 2x) + \frac{x \sin x}{4} + \frac{\cos 3x}{16} $$

14.
$$ \frac{d^4y}{dx^4} - 3 \frac{d^2y}{dx^2} - 4y = 5 \sin 2x - e^{-2x} \space \space; \space \space y(x) = c_1 e^{2x} + c_2 e^{-2x} + [c_3 \cos x + c_4 \sin x] + \frac{5 \sin 2x}{24} + \frac{xe^{-2x}}{20} $$

15.
$$ \frac{d^2y}{dx^2} - 2 \frac{dy}{dx} + 2y = \sinh x + \sin(\sqrt{2} \space x) \space \space; \space \space y(x) = e^x [c_1 \cos x + c_2 \sin x] + \frac{e^x}{2} - \frac{e^{-x}}{10} + \frac{\cos(\sqrt{2} \space x)}{2\sqrt{2}} $$

16.
$$ (D^4 - 3D^2 - 4)y = 24 \sin 2x - 40 e^{-2x} \space \space; \space \space y(x) = c_1 \cos x + c_2 \sin x + \sin 2x - 2x e^{-2x} $$

17.
$$ (D^3 + 1)y = \cos^2\left(\frac{x}{2}\right) + e^{-x} \space \space; \space \space y(x) = c_1 e^{-x} + e^{(x/2)} \left[c_2 \cos\left(\frac{\sqrt{3}}{2} x\right) + c_3 \sin\left(\frac{\sqrt{3}}{2} x\right)\right] + \frac{1}{2} + \frac{xe^{-x}}{3} + \frac{\cos x - \sin x}{4} $$


18.
$$ \frac{d^3y}{dt^3} + 3 \frac{d^2y}{dt^2} + \frac{dy}{dt} - 5y = \cosh t + \sin t \space \space; \space \space y(t) = c_1 e^t + e^{-2t} \left[c_2 \cos t + c_3 \sin t\right] + \frac{te^t}{20} - \frac{e^t}{8} - \frac{\sin t}{8} $$

19.
$$ \frac{d^2y}{dx^2} + 2 \frac{dy}{dx} + 2y = \sin 2x \cos 3x \space \space; \space \space y(x) = e^{-x} \left[c_1 \cos x + c_2 \sin x\right] + \frac{2 \cos x - \sin x}{10} - \frac{10 \cos(5x) + 23 \sin(5x)}{1258} $$

20.
$$ (D^2 + 2)y = x^3 \space \space; \space \space y(x) = c_1 \cos(\sqrt{2} \space x) + c_2 \sin(\sqrt{2} \space x) + \frac{x(x^2-3)}{2} $$

21.
$$ \frac{d^4y}{dx^4} + 4y = x^3 \space \space; \space \space y(x) = e^{-x} \left[c_1 \cos x + c_2 \sin x\right] + e^{x} \left[c_3 \cos x + c_4 \sin x\right] + \frac{x^3}{4} $$

22.
$$ \frac{d^2y}{dx^2} + \frac{dy}{dx} = x^2 + 2x + 4 \space \space; \space \space y(x) = c_1 + c_2 e^{-x} + \frac{x^3}{3} + 4x $$

23.
$$ (D^2 - 4D + 1)y = \cos 2x + x \space \space; \space \space y(x) = c_1 e^{(2 + \sqrt{3})x} + c_2 e^{(2 - \sqrt{3})x} + \frac{8 \sin 2x + 3 \cos 2x}{-73} + x + 4 $$

24.
$$ \frac{d^2y}{dx^2} - \frac{dy}{dx} + y = x^3 - 3x^2 + 1  \quad ; \quad y(x) = e^{(x/2)}\left[c_1 \cos\left(\frac{\sqrt{3}}{2} x\right) + c_2 \sin\left(\frac{\sqrt{3}}{2} x\right)\right] + x^3 + 6x - 5 $$

25.
$$ \frac{d^2y}{dx^2} - 2 \frac{dy}{dx} + y = e^x \sin 2x \space \space; \space \space y(x) = e^x \left[c_1 + c_2 x\right] + \frac{e^x \sin 2x}{-4} $$

26.
$$ \frac{d^2y}{dx^2} - y = e^x + x^2 e^x \space \space; \space \space y(x) = c_1 e^x + c_2 e^{-x} + \frac{xe^x}{2} + \frac{e^x}{2} \left( \frac{x^3}{3} - \frac{x^2}{2} + \frac{x}{2} \right) $$

27.
$$ \frac{d^3y}{dx^3} - 3 \frac{d^2y}{dx^2} + 3 \frac{dy}{dx} - y = e^x + xe^x \space \space; \space \space y(x) = e^x \left[c_1 + c_2 x + c_3 x^2\right] + \frac{x^3 e^x}{6} + \frac{e^x x^4}{24} $$

28.
$$ \frac{d^3y}{dx^3} - 7 \frac{d^2y}{dx^2} + 10 \frac{dy}{dx} = e^{2x} \sin x \space \space; \space \space y(x) = c_1 e^{2x} + c_2 e^{5x} + c_3 + \frac{e^{2x} (\sin x + 7 \cos x)}{50} $$

29.
$$ (D^4 + 4)y = e^x \sin^2 x \space \space; \space \space y(x) = c_1 \cos 2x + c_2 \sin 2x + \frac{e^x}{2} \left[ \frac{1}{5} + \frac{24 \sin 2x - 3 \cos 2x}{-585} \right] $$

30.
$$ (D^2 + 4)y = e^x \sin^2 x \space \space; \space \space y(x) = c_1 \cos 2x + c_2 \sin 2x + \frac{e^x}{2} \left[ \frac{1}{5} - \frac{4 \sin 2x + \cos 2x}{17} \right] $$

31.
$$ \frac{d^4y}{dx^4} - y = \cos x \cosh x \space \space; \space \space y(x) = c_1 e^x + c_2 e^{-x} + c_3 \cos x + c_4 \sin x - \frac{\cos x \cosh x}{5} $$

32.
$$ \frac{d^2y}{dx^2} + 5 \frac{dy}{dx} + 7y = e^{-2x} \sin 2x + x^2 \space \space; \space \space y(x) = e^{-\frac{5}{2} x} \left[c_1 \cos\left(\frac{\sqrt{3}}{2} x\right) + c_2 \sin\left(\frac{\sqrt{3}}{2} x\right)\right] - \frac{e^{-2x}}{13} (2 \cos 2x + 3 \sin 2x) + \frac{1}{49} (7x^2 + 10x + \frac{36}{7}) $$

33.
$$ \frac{d^2y}{dx^2} - y = x \sin x \space \space; \space \space y(x) = c_1 e^x + c_2 e^{-x} - \frac{x}{2} \sin x - \frac{\cos x}{2} $$

34.
$$ D^2 y - 2 D y + y = x e^x \sin x \space \space; \space \space y(x) = e^x \left[c_1 + c_2 x\right] - e^x \left[x \sin x + 2 \cos x\right] $$

35.
$$ \frac{d^2y}{dx^2} - 8 \frac{dy}{dx} + 20y = 40 \sin 4x \space \space; \space \space y(x) = e^{4x} \left[c_1 \cos 2x + c_2 \sin 2x\right] + \frac{2 \sin 4x + 16 \cos 4x}{13} $$

36.
$$ (D^2 + 2D + 5)y = 3^x \space \space; \space \space y(x) = e^{-x} \left[c_1 \cos 2x + c_2 \sin 2x\right] + \frac{3^x}{(\log 3)^2 + 2 \log 3 + 5} $$
